Did proofs for reverse (except mem)
Also changed order of theorem goals to be in order,
fix old tests (improve a few)

lib/Verif_List.v
@@ -1,4 +1,5 @@
 Require Import StdLib.
+Require Import Verif_Int.
 Require Import Lib_List.
 Set Bullet Behavior "Strict Subproofs".
 
@@ -130,26 +131,6 @@ Import Lib_Algebra.Algebra.
 Import Lib_Int.Int.
 Import Lib_List.List.
 
-
-(*TODO: move*)
-Require Import Verif_Int.
-Lemma length_int_list_ctx:
-  (theory_ctx_ext Length ++
-   theory_ctx_ext Int ++
-   (rec_fun app [:: l1; l2] app_body :: (theory_ctx_ext List ++ [::])%list)%SEQ) =
-[:: rec_fun length [:: l] length_body;
-nonrec_pred ge [:: Lib_Int.Int.x; Lib_Int.Int.y] ge_body;
-nonrec_pred le [:: Lib_Int.Int.x; Lib_Int.Int.y] le_body;
-nonrec_pred gt [:: Lib_Int.Int.x; Lib_Int.Int.y] gt_body;
-nonrec_fun sub [:: Lib_Int.Int.x; Lib_Int.Int.y] sub_body; 
-abs_pred lt; abs_fun mult; abs_fun plus; abs_fun neg;
-nonrec_fun one [::] (Tconst (ConstInt 1));
-nonrec_fun zero [::] (Tconst (ConstInt 0)); rec_fun app [:: l1; l2] app_body;
-nonrec_pred is_nil [:: l] is_nil_body; datatype_def list_mut].
-Proof.
-  reflexivity.
-Qed.
-
 End OtherCtx.
 
 (*Prove lemmas*)
@@ -174,99 +155,71 @@ Definition l1__ : term := Tfun (constsym "l1" list_a) nil nil.
 Definition l2__ : term := Tfun (constsym "l2" list_a) nil nil.
 Definition l3__ : term := Tfun (constsym "l3" list_a) nil nil.
 Definition l__ : term := Tfun (constsym "l" list_a) nil nil.
+Definition x__ : term := Tfun (constsym "x" a_) nil nil.
+Definition y__ : term := Tfun (constsym "y" a_) nil nil.
 
 Ltac extra_simpl ::= fold a_; fold x_; fold y_; 
   fold list_a;
   fold l1_; fold l2_; fold l3_; fold r_;
   unfold t_constsym;
   fold l1__; fold l2__; fold l3__; fold l__;
+  fold x__; fold y__;
   repeat (tryif progress(unfold ty_subst; try unfold ty_subst_var)
     then simpl else idtac).
 
-  Ltac wunfold_at x n :=
-  apply D_unfold_single with (f:=x)(i:=n); [prove_closed |];
-  unfold unfold_f_single; simpl; unfold unfold_f_single_aux; simpl;
-  unfold sub_fun_body_f, replace_tm_f, sub_body_t, safe_sub_ts; simpl;
-  repeat (progress(extra_simpl)).
 
-(*This is a hack, but unfolding the context
-  takes a long time. Instead we prove an equivalence*)
-
-
-(*Start with interesting ones (app, reverse)*)
+(*The interesting ones are Append and Reverse*)
 Lemma app_valid: valid_theory Append.
 Proof.
   simpl valid_theory.
-  split_all; auto; exists ["a"].
-  5: {
-    (*[app] is associative*)
-    (*Let's expand the context but NOT the assumptions (delta)*)
-    apply soundness.
-    simpl_task.
-    rewrite ListCtx.list_ctx. simpl.
-    rewrite ListAxioms.list_axioms. simpl.
+  split_all; auto; exists ["a"];
+  apply soundness; simpl_task;
+  rewrite ListCtx.list_ctx ListAxioms.list_axioms; simpl.
+  - (*[app] is associative*)
+    (*In all, we expand the context by rewriting,
+      not manually unfolding, which takes a long time*)
     simpl_mono.
     winduction.
-    - (*Nil case: simplify both sides*)
+    + (*Nil case: simplify both sides*)
       wintros "l2". wintros "l3".
-      wunfold_at app 0%N. 
-      wsimpl_match.
-      wunfold_at app 2%N.
-      wsimpl_match.
+      wunfold_at app 0%N; wsimpl_match.
+      wunfold_at app 2%N; wsimpl_match.
       wreflexivity.
-    - wintros "x" "l" "IH" "l2" "l3".
-      wunfold_at app 0%N.
-      wsimpl_match.
-      wunfold_at app 3%N.
-      wsimpl_match.
-      wunfold_at app 2%N.
-      wsimpl_match.
+    + wintros "x" "l" "IH" "l2" "l3".
+      wunfold_at app 0%N; wsimpl_match.
+      wunfold_at app 3%N; wsimpl_match.
+      wunfold_at app 2%N; wsimpl_match.
       (*Now we can rewrite with the IH*)
-      wf_equal. wreflexivity.
       wspecialize "IH" l2__ l3__.
       wrewrite "IH".
       wreflexivity.
-  }
-  4: {
-    (*l ++ nil = l*)
+  - (*l ++ nil = l*)
     (*This proof is much easier, it is almost the same
       as in Coq*)
-    apply soundness.
-    simpl_task.
-    rewrite ListCtx.list_ctx. simpl.
-    rewrite ListAxioms.list_axioms. simpl.
     simpl_mono.
     winduction.
-    - wunfold_at app 0%N. wsimpl_match.
+    + wunfold_at app 0%N; wsimpl_match.
       wreflexivity.
-    - wintros "x" "l" "IH".
-      wunfold_at app 0%N. wsimpl_match.
+    + wintros "x" "l" "IH".
+      wunfold_at app 0%N; wsimpl_match.
       wrewrite "IH".
       wreflexivity.
-  }
-  3: {
-    (*length (l1 ++ l2) = length l1 + length l2*)
-    apply soundness.
-    simpl_task.
-    (*simplify context by rewriting because unfolding takes forever*)
-    rewrite ListCtx.length_ctx.
-    rewrite Verif_Int.IntCtx.int_ctx.
-    rewrite ListCtx.list_ctx. simpl.
-    (*Simplify delta*)
-    rewrite ListAxioms.length_axioms.
-    rewrite ListAxioms.list_axioms.
-    rewrite Verif_Int.IntCtx.int_axioms.
-    simpl.
+  - (*length (l1 ++ l2) = length l1 + length l2*)
+    (*Here, we cannot unfold even if we wanted to*)
+    rewrite ListCtx.length_ctx 
+    Verif_Int.IntCtx.int_ctx
+    ListAxioms.length_axioms
+    Verif_Int.IntCtx.int_axioms; simpl.
     simpl_mono.
     winduction.
-    - wintros "l2". wunfold_at app 0%N. wsimpl_match.
-      wunfold_at length 1%N.
-      wsimpl_match.
+    + wintros "l2". 
+      wunfold_at app 0%N; wsimpl_match.
+      wunfold_at length 1%N; wsimpl_match.
       (*Use fact that x + 0 = x*)
       wspecialize "Unit_def_l" <t length<a_>(l2__) t>.
       wrewrite "Unit_def_l".
       wreflexivity.
-    - (*Inductive case*)
+    + (*Inductive case*)
       wintros "x" "l" "IH" "l2".
       wunfold_at app 0%N; wsimpl_match.
       wunfold_at length 0%N; wsimpl_match.
@@ -278,9 +231,104 @@ Proof.
         <t length<a_>(l2__) t>.
       wrewrite "Assoc".
       wreflexivity.
-  }
   (*We do not (yet) do the mem goals*)
   (*TODO: do predicate unfolding then this*)
-  admit.
-  admit.
+  - admit.
+  - admit.
 Admitted.
+
+(*Reverse*)
+Lemma rev_valid: valid_theory Reverse.
+Proof.
+  simpl valid_theory.
+  split_all; auto; exists ["a"];
+  apply soundness; simpl_task;
+  rewrite ListCtx.list_ctx ListAxioms.list_axioms
+  ListCtx.app_ctx ListAxioms.app_axioms
+  ListCtx.mem_ctx ListAxioms.mem_axioms
+  ListCtx.length_ctx ListAxioms.length_axioms
+  Verif_Int.IntCtx.int_ctx Verif_Int.IntCtx.int_axioms ; simpl.
+  - simpl_mono.
+    (*Don't need induction here*)
+    wintros "l1" "l2" "x".
+    wunfold_at reverse 0%N; wsimpl_match.
+    (*Use app_assoc*)
+    (*Need to specialize type*)
+    wspecialize_ty "Append_assoc" [("a", a_)].
+    wspecialize "Append_assoc" <t reverse <a_>(l1__) t>
+      <t Cons<a_>(x__, Nil<a_>()) t>
+      l2__.
+    wrewrite<- "Append_assoc".
+    wunfold_at app 1%N; wsimpl_match.
+    wunfold_at app 1%N; wsimpl_match.
+    wreflexivity.
+  - (*reverse_cons is even easier*)
+    simpl_mono.
+    wintros "l" "x".
+    wunfold_at reverse 0%N; wsimpl_match.
+    wreflexivity.
+  - (*cons_reverse now needs induction*)
+    simpl_mono.
+    winduction.
+    + wintros "x".
+      wunfold_at reverse 0%N; wsimpl_match.
+      wunfold app; wsimpl_match.
+      wunfold reverse; wsimpl_match.
+      wunfold reverse; wsimpl_match.
+      wunfold app; wsimpl_match.
+      wreflexivity.
+    + wintros "x" "l" "IH" "y".
+      wunfold app; wsimpl_match.
+      wunfold_at reverse 1%N; wsimpl_match.
+      wspecialize "IH" y__.
+      wrewrite<- "IH".
+      wunfold app; wsimpl_match.
+      (*Now use [reverse_cons]*)
+      wspecialize_ty "reverse_cons" [("a", a_)].
+      wspecialize "reverse_cons" l__ x__.
+      wrewrite "reverse_cons".
+      wreflexivity.
+  - (*reverse_reverse follows from these*)
+    simpl_mono.
+    winduction.
+    + wunfold_at reverse 1%N; wsimpl_match.
+      wunfold reverse; wsimpl_match.
+      wreflexivity.
+    + wintros "x" "l" "IH".
+      wunfold_at reverse 1%N; wsimpl_match.
+      (*Use cons_reverse here*)
+      wspecialize_ty "cons_reverse" [("a", a_)].
+      wspecialize "cons_reverse" <t reverse<a_>(l__) t> x__.
+      wrewrite<- "cons_reverse".
+      wrewrite "IH".
+      wreflexivity.
+  - (*TODO: mem*) admit.
+  - (*length of reverse - from length_app*)
+    simpl_mono.
+    winduction.
+    + wunfold reverse; wsimpl_match.
+      wreflexivity.
+    + wintros "x" "l" "IH".
+      wunfold reverse; wsimpl_match.
+      (*Use Append_length*)
+      wspecialize_ty "Append_length" [("a", a_)].
+      wspecialize "Append_length" <t reverse<a_>(l__) t>
+        <t Cons<a_>(x__, Nil<a_>()) t>.
+      wrewrite "Append_length".
+      wrewrite "IH".
+      do 3 (wunfold_at length 1%N ; wsimpl_match).
+      (*Now, just some int arithemtic*)
+      wassert "Honezero" <f [int] plus(one(), zero()) = one() f>.
+      {
+        wspecialize "Comm" <t one() t> <t zero() t>.
+        wrewrite "Comm".
+        wspecialize "Unit_def_l" <t one() t>.
+        wassumption.
+      }
+      wrewrite "Honezero".
+      wspecialize "Comm"  <t length<a_>(l__) t>
+        <t one() t>.
+      wassumption.
+Admitted.
+
+End ListProofs.
